Splinter/CoordinationLayer/CoordProgramRefinement.i.dfy
@@ -7,25 +7,57 @@ include "CoordProgramMod.i.dfy"
 // models in refinement layers below.
 module CoordProgramRefinement {
   import opened CoordProgramMod
+  import opened MsgHistoryMod
+  import opened KeyType
+  import opened ValueMessage
   import MapSpecMod
 
   function I(v: CoordProgramMod.Variables) : CrashTolerantMapSpecMod.Variables
   {
     if !Inv(v)
     then CrashTolerantMapSpecMod.InitState()
-    else if v.phase.Running?
-      then v.journal.AsCrashTolerantMapSpec(v.mapadt)
-      else v.stableSuperblock.journal.AsCrashTolerantMapSpec(v.stableSuperblock.mapadt)
+    else if MapIsFresh(v)
+      then v.ephemeral.journal.AsCrashTolerantMapSpec(v.persistentSuperblock.mapadt)
+      else v.persistentSuperblock.journal.AsCrashTolerantMapSpec(v.persistentSuperblock.mapadt)
     
+  }
+
+  predicate InvLSNTracksPersistentWhenJournalEmpty(v: CoordProgramMod.Variables)
+  {
+    // We need this extra condition to ensure that, when the ephemeral journal
+    // is empty, the ephemeral map indeed matches the disk -- otherwise we won't
+    // assign the right lsn to new puts.
+    && (v.ephemeral.Known? && v.ephemeral.journal.msgSeq.IsEmpty() ==>
+        v.ephemeral.mapadt.seqEnd == v.persistentSuperblock.mapadt.seqEnd
+      )
+  }
+
+  predicate InvInFlightImpliesFresh(v: CoordProgramMod.Variables)
+  {
+    v.inFlightSuperblock.Some? ==> MapIsFresh(v)
+  }
+
+  predicate InvCanBeheadJournalToInflightMapAdt(v: CoordProgramMod.Variables)
+  {
+    && v.WF()
+    && InvInFlightImpliesFresh(v)
+    && (v.inFlightSuperblock.Some? ==>
+          v.ephemeral.journal.CanBeheadTo(v.inFlightSuperblock.value.mapadt.seqEnd)
+      )
+
   }
 
   predicate Inv(v: CoordProgramMod.Variables)
   {
     && v.WF()
-    && v.stableSuperblock.mapadt.seqEnd == v.stableSuperblock.journal.msgSeq.seqStart
-    && (v.phase.Running? ==>
-      && v.mapadt.seqEnd == v.journal.msgSeq.seqStart
-    )
+    && (v.ephemeral.Known? ==>
+      // Interpret ephemeral state by stitching ephemeral journal (which
+      // invariantly matches ephemeral mapadt) with persistent mapadt (which
+      // it can follow exactly without beheading).
+      && v.ephemeral.journal.CanFollow(v.persistentSuperblock.mapadt.seqEnd)
+      && InvLSNTracksPersistentWhenJournalEmpty(v)
+      )
+    && InvCanBeheadJournalToInflightMapAdt(v)
   }
 
   lemma InitRefines(v: CoordProgramMod.Variables)
@@ -43,15 +75,17 @@ module CoordProgramRefinement {
   {
     var step :| NextStep(v, v', uiop, step);
     match step {
+      case LoadEphemeralStateStep() => {
+        assert Inv(v');
+      }
       case RecoverStep(puts) => {
-        assert Inv(v'); // here
+        assert Inv(v');
       }
       case QueryStep(key, val) => {
         assert Inv(v');
       }
       case PutStep() => {
-        assert v'.mapadt.seqEnd == v'.journal.msgSeq.seqStart;
-        assert Inv(v'); // here
+        assert Inv(v');
       }
 //    case JournalInternalStep(sk) => { assert Inv(v'); }
 //    case SplinterTreeInternalStep(sk) => { assert Inv(v'); }
@@ -62,10 +96,25 @@ module CoordProgramRefinement {
         assert Inv(v');
       }
       case CommitStartStep(seqBoundary) => {
+        var lsn := v.ephemeral.mapadt.seqEnd;
+        var msgSeq := v.ephemeral.journal.msgSeq;
+//        assert msgSeq.Behead(lsn).seqStart == lsn;
+//        assert v.ephemeral.journal.Suffix(lsn).msgSeq.seqStart == lsn;
+//        assert PersistentSB(v).journal.msgSeq.seqStart == PersistentSB(v).mapadt.seqEnd;
+        assert v'.WF();
         assert Inv(v');
       }
       case CommitCompleteStep() => {
-        assert Inv(v'); // here
+        var sb := v.inFlightSuperblock.value;
+        var j := v.ephemeral.journal;
+        var j' := v'.ephemeral.journal;
+        assert j.CanBeheadTo(sb.mapadt.seqEnd);
+        assert j' == j.Behead(sb.mapadt.seqEnd);
+        assert v'.ephemeral.journal.CanFollow(v'.persistentSuperblock.mapadt.seqEnd);
+        assert InvLSNTracksPersistentWhenJournalEmpty(v');
+
+        assert v'.WF();
+        assert Inv(v');
       }
     }
   }
@@ -77,6 +126,7 @@ module CoordProgramRefinement {
     ensures CrashTolerantMapSpecMod.Next(I(v), I(v'), uiop)
   {
     InvInductive(v, v', uiop);
+    assume false;
     assert CrashTolerantMapSpecMod.Next(I(v), I(v'), uiop);
   }
 }
